theories/lang/cpp/specs.v
@@ -6,4 +6,5 @@
 From bedrock.lang.cpp.specs Require Export
      with_pre_post
      functions
-     spec_notations.
+     cpp_specs
+     elaborate.
